\DocumentMetadata{tagging = on}
\documentclass{ltx-talk}

\setmainfont{Pennstander-Regular.otf}
\setmathfont{PennstanderMath-Regular.otf}


\begin{document}

\begin{frame}
  \frametitle{The Quadratic Formula}

  \Huge
  \[
    ax^2+bx+c=0
  \]


  
\end{frame}


\begin{frame}
  \frametitle{Completing the Square}

  \large

  First, complete the square
  
  \begin{itemize}[action-spec=<+->,item-vspace=20pt,begin-vspace=20pt]
  \item  $ax^2+bx+c=0$
  \item  $x^2+\frac{b}{a}x+\frac{c}{a}=0$
  \item  $x^2+\frac{b}{a}x+\bigl(\frac{b}{2a}\bigr)^2=-\frac{c}{a}+\bigl(\frac{b}{2a}\bigr)^2$
  \item  $\bigl(x+\frac{b}{2a}\bigr)^2=-\frac{c}{a}+\bigl(\frac{b}{2a}\bigr)^2$
  \end{itemize}
\end{frame}

\begin{frame}
 \frametitle{Solve for $x$}
 \large

 Now, solve for $x$
 
  \begin{itemize}[action-spec=<+->,item-vspace=20pt,begin-vspace=20pt]
  \item $\bigl(x+\frac{b}{2a}\bigr)^2=-\frac{c}{a}+\bigl(\frac{b}{2a}\bigr)^2$
  \item $x+\bigl(\frac{b}{2a}\bigr)=\pm\sqrt{-\frac{c}{a}+\bigl(\frac{b}{2a}\bigr)^2}$
 \item $x=-\bigl(\frac{b}{2a}\bigr)\pm\sqrt{-\frac{c}{a}+\bigl(\frac{b}{2a}\bigr)^2}$
  \item $\displaystyle x=\frac{-b\pm\sqrt{b^2-4ac}}{2a}$
  \end{itemize}
    
\end{frame}

\begin{frame}
 \frametitle{The Quadratic Formula}
 \large

 The solution of the quadratic equation.

 \[ax^2+bx+x=0\]

 where $a$ is non zero, is given by the formula

  \[x=\frac{-b\pm\sqrt{b^2-4ac}}{2a}\]

    
\end{frame}

\end{document}
